proof/refine/AARCH64/ADT_H.thy
@@ -109,12 +109,11 @@ definition absHeapArch ::
          Some (AARCH64_A.ASIDPool (\<lambda>w. map_option abs_asid_entry (ap (ucast w))))
      | KOPTE _ \<Rightarrow>
          map_option PageTable (absPageTable h (pt_types a) a)
-     | KOVCPU (VCPUObj tcb vgic regs vppimask vtimer) \<Rightarrow>
+     | KOVCPU (VCPUObj tcb vgic regs vppimask) \<Rightarrow>
        Some (VCPU \<lparr> vcpu_vgic   = absVGIC vgic,
                     vcpu_regs   = regs,
                     vcpu_tcb    = tcb,
-                    vcpu_vppi_masked = vppimask,
-                    vcpu_vtimer = vtimer \<rparr>)"
+                    vcpu_vppi_masked = vppimask \<rparr>)"
 
 definition
   "EndpointMap ep \<equiv> case ep of
