proof/refine/AARCH64/CNodeInv_R.thy
@@ -9117,22 +9117,20 @@ crunch vcpuUpdate, vcpuWriteReg, vcpuSaveReg, vcpuRestoreReg, vcpuReadReg
 lemma saveVirtTimer_irq_states'[wp]:
   "saveVirtTimer vcpu_ptr \<lbrace>valid_irq_states'\<rbrace>"
   unfolding saveVirtTimer_def
-  by (wpsimp simp: read_cntpct_def
-             wp: doMachineOp_irq_states')
+  by (wpsimp wp: doMachineOp_irq_states')
 
 lemma restoreVirtTimer_irq_states'[wp]:
   "restoreVirtTimer vcpu_ptr \<lbrace>valid_irq_states'\<rbrace>"
   unfolding restoreVirtTimer_def isIRQActive_def
-  by (simp add: liftM_bind)
-     (wpsimp wp: maskInterrupt_irq_states' getIRQState_wp hoare_vcg_imp_lift' doMachineOp_irq_states'
-             simp: if_apply_def2 read_cntpct_def)
+  by (wpsimp wp: maskInterrupt_irq_states' getIRQState_wp
+             simp: if_apply_def2 liftM_bind)
 
 crunch
   vcpuDisable, vcpuEnable, vcpuRestore, vcpuRestoreReg, vcpuSaveReg,
   vcpuUpdate, vgicUpdateLR, vcpuSave
   for irq_states' [wp]: valid_irq_states'
   (wp: crunch_wps maskInterrupt_irq_states'[where b=True, simplified] no_irq no_irq_mapM_x
-   simp: crunch_simps no_irq_isb no_irq_dsb no_irq_modify
+   simp: crunch_simps no_irq_modify
          set_gic_vcpu_ctrl_hcr_def setSCTLR_def setHCR_def get_gic_vcpu_ctrl_hcr_def
          getSCTLR_def get_gic_vcpu_ctrl_lr_def get_gic_vcpu_ctrl_apr_def
          get_gic_vcpu_ctrl_vmcr_def
